coq: ZF: Class.Isom.IsomFromTransport

coq/ZF/Class/Isom.v
@@ -13,6 +13,7 @@ Require Import ZF.Set.OrdPair.
 Definition Isom (F R S A B:Class) : Prop := Bij F A B /\ forall x y, A x -> A y ->
   R :(x,y): <-> S :(F!x,F!y):.
 
+(* An isomorphism is a bijection.                                               *)
 Proposition IsomIsBij : forall (F R S A B:Class),
   Isom F R S A B -> Bij F A B.
 Proof.
@@ -56,3 +57,35 @@ Proof.
       * rewrite (BijComposeEval F G A B C x) in H7; try assumption.
         rewrite (BijComposeEval F G A B C y) in H7; try assumption.
 Qed.
+
+(* Transporting a 'relation R on A' by F.                                       *)
+Definition transport (F R A:Class) : Class := fun x =>
+  exists y z, x = :(F!y,F!z): /\ A y /\ A z /\ R :(y,z):.
+
+Proposition TransportCharac2F : forall (F R A B:Class) (y z:U),
+  Bij F A B ->
+  A y       ->
+  A z       ->
+  transport F R A :(F!y,F!z): <-> A y /\ A z /\ R :(y,z):.
+Proof.
+  intros F R A B y z H1 H2 H3. split; intros H4.
+  - destruct H4 as [y' [z' [H4 [H5 [H6 H7]]]]]. apply OrdPairEqual in H4.
+    destruct H4 as [H4 H8].
+    assert (y = y') as H9.  { apply BijEvalInjective with F A B; assumption. }
+    assert (z = z') as H10. { apply BijEvalInjective with F A B; assumption. }
+    subst. split. 1: assumption. split; assumption.
+  - destruct H4 as [H4 [H5 H6]]. exists y. exists z. split.
+    1: reflexivity. split. 1: assumption. split; assumption.
+Qed.
+
+Proposition IsomFromTransport : forall (F R S A B:Class),
+  (S = transport F R A) -> Bij F A B -> Isom F R S A B.
+Proof.
+  intros F R S A B H1 H2. split. 1: assumption.
+  intros x y H3 H4. split; intros H5.
+  - rewrite H1. apply (TransportCharac2F F R A B); try assumption.
+    split. 1: assumption. split; assumption.
+  - rewrite H1 in H5. apply (TransportCharac2F F R A B) in H5; try assumption.
+    destruct H5 as [_ [_ H5]]. assumption.
+Qed.
+
